cheririscV/CapMemtype.v
@@ -158,7 +158,7 @@ interface *)
   pair [(m', b)] of the updated memory state [m'] and the identifier
   [b] of the newly-allocated block.  Note that [alloc] never fails: we
   are modeling an infinite memory. Alloc only allocates heap memory *)
-Parameter alloc: forall (m: mem) (c: compartment) (len: nat), pointer * mem + error_kind.
+Parameter alloc: forall (m: mem) (cap: occap) (c: compartment) (len: nat), pointer * mem + error_kind.
 
 (** [free m b lo hi cp] frees (deallocates) the range of offsets from [lo]
   included to [hi] excluded in block [b], which must be owned by
@@ -238,7 +238,7 @@ Parameter drop_perm: forall (m: mem) (c: occap) (p: permission) (cp: compartment
 (** [block_compartment m c] returns the list of heap capabilities internal to
     compartment [c] *)
 
-Parameter block_compartment: forall (m: mem) (c: compartment), occap.
+Parameter block_compartment: forall (m: mem) (c: compartment), list occap.
 
 (** [perm m b ofs k p] holds if the address [b, ofs] in memory state [m]
   has permission [p]: one of freeable, writable, readable, and nonempty.
@@ -289,7 +289,7 @@ Axiom disjoint_cap_dec: forall c c', {disjoint_cap c c'} + {~ disjoint_cap c c'}
 Definition can_access_block (m: mem) (c: occap) (cp: option compartment): Prop :=
   match cp with
   | None => True
-  | Some cp => derived_cap (block_compartment m cp) c
+  | Some cp => Exists (fun cap => derived_cap cap c) (block_compartment m cp)
   end.
 
 (** [max_read_auth c] derives the maximal read authority of a
@@ -825,16 +825,16 @@ Axiom storebytes_concat:
 (** Effect of [alloc] on permissions. *)
 
 Axiom perm_alloc_1:
-  forall m1 c len m2 ptr, alloc m1 c len = inl (ptr,m2) ->
+  forall m1 cap c len m2 ptr, alloc m1 cap c len = inl (ptr,m2) ->
   forall ofs k p, perm m1 ofs k p -> perm m2 ofs k p.
 Axiom perm_alloc_2:
-  forall m1 c l m2 ptr, alloc m1 c l = inl (ptr,m2) ->
-  let lo_ofs := Ptrofs.unsigned (get_lo (block_compartment m2 c)) in
+  forall m1 cap c l m2 ptr, alloc m1 cap c l = inl (ptr,m2) ->
+  let lo_ofs := Ptrofs.unsigned (get_lo cap) in
   let ptr_ofs := Ptrofs.unsigned (pointer_ofs ptr) in
   forall ofs k, lo_ofs + ptr_ofs <= ofs < lo_ofs + ptr_ofs + Z.of_nat l ->
            perm m2 ofs k Freeable.
 Axiom perm_alloc_inv:
-  forall m1 c l m2 ptr, alloc m1 c l = inl (ptr,m2) ->
+  forall m1 cap c l m2 ptr, alloc m1 cap c l = inl (ptr,m2) ->
   forall ofs k p,
   perm m2 ofs k p ->
   Ptrofs.unsigned (pointer_ofs ptr) <= ofs < (Ptrofs.unsigned (pointer_ofs ptr) + Z.of_nat l) \/ perm m1 ofs k p.
@@ -842,23 +842,21 @@ Axiom perm_alloc_inv:
 (** Effect of [alloc] on compartments. *)
 
 Axiom alloc_block_compartment:
-  forall m1 c l m2 ptr,
-    alloc m1 c l = inl (ptr,m2) ->
-    Ptrofs.unsigned (get_lo (block_compartment m2 c))
-    <= Ptrofs.unsigned (Ptrofs.add (get_lo (block_compartment m2 c)) (pointer_ofs ptr))
-    < Ptrofs.unsigned (get_hi (block_compartment m2 c)).
+  forall m1 cap c l m2 ptr,
+    alloc m1 cap c l = inl (ptr,m2) ->
+    Ptrofs.unsigned (get_lo cap)
+    <= Ptrofs.unsigned (Ptrofs.add (get_lo cap) (pointer_ofs ptr))
+    < Ptrofs.unsigned (get_hi cap).
 
 (** Effect of [alloc] on access validity. *)
 
 Axiom valid_access_alloc_other:
-  forall m1 c l m2 ptr, alloc m1 c l = inl (ptr,m2) ->
+  forall m1 cap c l m2 ptr, alloc m1 cap c l = inl (ptr,m2) ->
   forall k' chunk ptr' ofs' p cp' o ptr'',
   valid_access k' m1 chunk ptr' ofs' p cp' o ptr'' ->
   valid_access k' m2 chunk ptr' ofs' p cp' o ptr''.
 Axiom valid_access_alloc_same:
-  forall m1 c l m2 ptr,
-    alloc m1 c l = inl (ptr,m2) ->
-   let cap := block_compartment m2 c in
+  forall m1 cap c l m2 ptr, alloc m1 cap c l = inl (ptr,m2) ->
    let ofs := Ptrofs.unsigned (pointer_ofs ptr) in
    let ptr'' := Some cap in
    forall chunk o,
@@ -867,11 +865,10 @@ Axiom valid_access_alloc_same:
     (align_chunk chunk | derive_offset DEFAULT cap ofs) ->
     valid_access DEFAULT m2 chunk cap ofs Freeable (Some c) o ptr''.
 Axiom valid_access_alloc_inv:
-  forall m1 c l m2 ptr,
-    alloc m1 c l = inl (ptr,m2) ->
+  forall m1 cap c l m2 ptr, alloc m1 cap c l = inl (ptr,m2) ->
     forall k chunk ptr' p c' o ptr'' ofs,
       valid_access k m2 chunk ptr' ofs p c' o ptr'' ->
-      if derived_cap_dec (block_compartment m2 c) ptr'
+      if derived_cap_dec cap ptr'
       then in_bounds k ptr' ofs (size_chunk_nat chunk)
            /\ (align_chunk chunk | (derive_offset k ptr' ofs))
            /\ dynamic_conditions m2 k ptr' ofs (size_chunk chunk) o (Some c) ptr''
@@ -880,16 +877,14 @@ Axiom valid_access_alloc_inv:
 (** Load-alloc properties. *)
 
 Axiom load_alloc_unchanged:
-  forall m1 c l m2 ptr,
-    alloc m1 c l = inl (ptr,m2) ->
+  forall m1 cap c l m2 ptr, alloc m1 cap c l = inl (ptr,m2) ->
     forall k chunk ptr' ofs' c' ,
-      disjoint_cap (block_compartment m2 c) ptr' ->
+      disjoint_cap cap ptr' ->
       load k chunk m2 ptr' ofs' c' = load k chunk m1 ptr' ofs' c'.
 Axiom load_alloc_same:
-  forall m1 c l m2 ptr,
-    alloc m1 c l = inl (ptr,m2) ->
+  forall m1 cap c l m2 ptr, alloc m1 cap c l = inl (ptr,m2) ->
     forall chunk v,
-      load DEFAULT chunk m2 (block_compartment m2 c) (Ptrofs.unsigned (pointer_ofs ptr)) (Some c) = inl v ->
+      load DEFAULT chunk m2 cap (Ptrofs.unsigned (pointer_ofs ptr)) (Some c) = inl v ->
       v = OCVundef.
 (* Axiom load_alloc_same': *)
 (*   forall m1 c l m2 ptr, *)
@@ -901,8 +896,7 @@ Axiom load_alloc_same:
 (*       load k chunk m2 ptr' ofs (Some c) = inl OCVundef. *)
 
 Axiom load_alloc_other:
-  forall m1 c l m2 ptr,
-    alloc m1 c l = inl (ptr,m2) ->
+  forall m1 cap c l m2 ptr, alloc m1 cap c l = inl (ptr,m2) ->
     forall k chunk ptr' ofs c' v,
   load k chunk m1 ptr' ofs c' = inl v ->
   load k chunk m2 ptr' ofs c' = inl v.
